theories/AlmostStlc/Types.v
@@ -4,6 +4,7 @@ Inductive type : Type :=
   | Nat : type
   | List : type -> type
   | Pair : type -> type -> type
+  | Sum : type -> type -> type
   | Arrow : type -> (list (list (type * type))) -> type -> type
 .
 Notation ctx := (list type).
@@ -20,6 +21,7 @@ Section type_mutind.
   Context (HNat : Pt Nat).
   Context (HList : forall t : type, Pt t -> Pt (List t)).
   Context (HPair : forall t1 t2, Pt t1 -> Pt t2 -> Pt (Pair t1 t2)).
+  Context (HSum : forall t1 t2, Pt t1 -> Pt t2 -> Pt (Sum t1 t2)).
   Context (HArrow : forall t1 MR t2, Pt t1 -> Pmfix MR -> Pt t2 -> Pt (Arrow t1 MR t2)).
   Context (Hnil1 : Pmfix nil) (Hcons1 : forall R MR, Pcall R -> Pmfix MR -> Pmfix (cons R MR)).
   Context (Hnil2 : Pcall nil) (Hcons2 : forall t1 t2 R, Pt t1 -> Pt t2 -> Pcall R -> Pcall (cons (t1, t2) R)).
@@ -29,6 +31,7 @@ Section type_mutind.
       type_mutind Nat := HNat;
       type_mutind (List t) := HList t (type_mutind t);
       type_mutind (Pair t1 t2) := HPair t1 t2 (type_mutind t1) (type_mutind t2);
+      type_mutind (Sum t1 t2) := HSum t1 t2 (type_mutind t1) (type_mutind t2);
       type_mutind (Arrow t1 MR t2) := HArrow t1 MR t2 (type_mutind t1) (mfix_mutind MR) (type_mutind t2);
     }
    where mfix_mutind (MR : mfix_ctx) : Pmfix MR :=
